examples/Auto/AutoProver.v
@@ -65,7 +65,7 @@ Section parameterized.
 
   Variable hints : Hints.
 
-   Fixpoint openOver (e : expr func) (skip add : nat) : expr func :=
+  Fixpoint openOver (e : expr func) (skip add : nat) : expr func :=
     match e with
       | Var v =>
         if v ?[ lt ] skip then Var v
@@ -116,117 +116,42 @@ Section parameterized.
         exprD' (tus ++ tvs') tvs (openOver e (length tvs) (length tus)) t = Some val' /\
         forall us vs, val us (HList.hlist_app vs vs') = val' (HList.hlist_app us vs') vs.
   Proof.
-(*
     clear. induction e; simpl; intros.
     { consider (v ?[ lt ] length tvs); intros.
-      { generalize (@exprD'_Var_App_L _ _ _ us tvs' t tvs v H0).
+      { generalize (@exprD'_Var_App_L _ _ _ tus tvs' t tvs v H0).
         rewrite H. intros; forward.
-        red_exprD. forward. rewrite H1.
-        eauto. }
+        red_exprD. forward.
+        subst. eexists; split; eauto. intros.
+        inv_all; subst. auto. }
       { red_exprD.
-        eexists. split.
-        2: reflexivity.
-        unfold EnvI.lookupAs.
-        rewrite ListNth.nth_error_app_R by omega.
-        replace (v - length tvs + length us - length us) with (v - length tvs) by omega.
-        revert H. gen_refl.
-        pattern (nth_error (tvs ++ tvs') v) at 1 3.
-        destruct (nth_error (tvs ++ tvs') v); try congruence.
-        intros; forward. inv_all; subst.
-        assert (nth_error tvs' (v - length tvs) = Some t).
-        { rewrite ListNth.nth_error_app_R in e; eauto. omega. }
-        generalize H.
-        eapply  nth_error_join_env in H. intro.
-        destruct H. rewrite H.
-        simpl. red_exprD.
-        f_equal.
-        apply functional_extensionality.
-        intros.
-        rewrite HList.hlist_nth_hlist_app; eauto with typeclass_instances.
-        cut (nth_error tvs v = None); intros.
-        { gen_refl.
-          generalize dependent (HList.cast1 tvs tvs' v).
-          generalize dependent (HList.cast2 tvs tvs' v).
-          change (let ZZZ := (HList.hlist_nth x0 v) in forall
-                    (e0 : nth_error tvs v = None ->
-                          nth_error tvs' (v - length tvs) = nth_error (tvs ++ tvs') v)
-                    (e1 : forall v0 : typ,
-                            nth_error tvs v = Some v0 -> Some v0 = nth_error (tvs ++ tvs') v)
-                    (e2 : nth_error tvs v = nth_error tvs v),
-                    x =
-                    match
-                      e in (_ = t'')
-                      return
-                      (match t'' with
-                         | Some t0 => typD ts nil t0
-                         | None => unit
-                       end -> typD ts nil t)
-                    with
-                      | eq_refl => fun x1 : typD ts nil t => x1
-                    end
-                      (match
-                          nth_error tvs v as k
-                          return
-                          (nth_error tvs v = k ->
-                           match nth_error (tvs ++ tvs') v with
-                             | Some t0 => typD ts nil t0
-                             | None => unit
-                           end)
-                        with
-                          | Some i =>
-                            fun pf : nth_error tvs v = Some i =>
-                              match
-                                e1 i pf in (_ = z)
-                                return
-                                (match nth_error tvs v with
-                                   | Some t0 => typD ts nil t0
-                                   | None => unit
-                                 end ->
-                                 match z with
-                                   | Some t0 => typD ts nil t0
-                                   | None => unit
-                                 end)
-                              with
-                                | eq_refl =>
-                                  match
-                                    eq_sym pf in (_ = w)
-                                    return
-                                    (match w with
-                                       | Some t0 => typD ts nil t0
-                                       | None => unit
-                                     end -> typD ts nil i)
-                                  with
-                                    | eq_refl => fun x1 : typD ts nil i => x1
-                                  end
-                              end ZZZ
-                          | None =>
-                            fun pf : nth_error tvs v = None =>
-                              match
-                                e0 pf in (_ = z)
-                                return
-                                match z with
-                                  | Some t0 => typD ts nil t0
-                                  | None => unit
-                                end
-                              with
-                                | eq_refl => HList.hlist_nth vs' (v - length tvs)
-                              end
-                        end e2)).
-          intro. clearbody ZZZ. revert ZZZ.
-          rewrite H2. intros.
-          generalize (e0 e2).
-          generalize dependent (nth_error (tvs ++ tvs') v).
-          intros; subst.
-          eapply EnvI.split_env_nth_error in H.
-          rewrite EnvI.split_env_join_env in *. simpl in *.
+        forward. inv_all; subst.
+        eapply nth_error_get_hlist_nth_appR in H1; eauto with typeclass_instances. 2: omega.
+        destruct H1.
+        simpl in *.
+        match goal with
+          | |- context [ match ?X with _ => _ end ] =>
+            consider X
+        end; intros.
+        { destruct s. simpl in *.
+          eapply nth_error_get_hlist_nth_appR in H1; eauto with typeclass_instances. 2: omega.
+          simpl in *. forward_reason.
+          replace (v - length tvs + length tus - length tus) with (v - length tvs) in * by omega.
+          simpl in *.
           match goal with
-            | _ : _ ?X |- _ = match _ with eq_refl => ?Y end =>
-              change Y with X; generalize dependent X
+            | H : ?X = _ , H' : ?Y = _ |- _ =>
+              change Y with X in H' ; rewrite H in H'
           end.
-          clear - H1. revert e4. rewrite H1. intros.
-          uip_all.
-          inv_all; subst. reflexivity. }
-        { apply ListNth.nth_error_past_end. omega. } } }
+          inv_all. subst.
+          rewrite typ_cast_typ_refl.
+          eexists; split; eauto. simpl.
+          intros. rewrite H2. auto. }
+        { exfalso.
+          apply ExprDI.nth_error_get_hlist_nth_None in H1.
+          rewrite ListNth.nth_error_app_R in H1 by omega.
+          replace (v - length tvs + length tus - length tus) with (v - length tvs) in * by omega.
+          destruct H.
+          eapply ExprDI.nth_error_get_hlist_nth_Some in H.
+          destruct H. simpl in *. congruence. } } }
     { red_exprD.
       forward.
       inv_all; subst.
@@ -234,9 +159,6 @@ Section parameterized.
     { red_exprD.
       forward. inv_all; subst.
       eapply openOver_typeof_expr in H0.
-      rewrite typeof_env_app.
-      rewrite EnvI.typeof_env_join_env.
-      rewrite typeof_env_length in *.
       rewrite H0.
       specialize (IHe1 _ _ _ _ H1 vs').
       specialize (IHe2 _ _ _ _ H2 vs').
@@ -260,10 +182,13 @@ Section parameterized.
       rewrite <- H0. simpl. reflexivity. }
     { red_exprD.
       forward. inv_all; subst.
-      eapply EnvI.lookupAs_weaken in H.
-      rewrite H. eauto. }
+      eapply ExprDI.nth_error_get_hlist_nth_weaken with (ls' := tvs') in H0.
+      simpl in *.
+      forward_reason.
+      rewrite H.
+      rewrite typ_cast_typ_refl.
+      eexists; split; eauto. simpl. intros. eauto. }
   Qed.
-*) Admitted.
 
   Definition applicable (s : subst) (tus tvs : EnvI.tenv typ)
              (lem : lemma func (expr func)) (e : expr func)
